new extraction

openmls/src/binary_tree/array_representation/treemath.rs
@@ -38,14 +38,17 @@ impl std::fmt::Display for LeafNodeIndex {
 
 #[attributes]
 impl LeafNodeIndex {
-    /// Create a new `LeafNodeIndex` from a `u32`.
-    pub fn new(index: u32) -> Self {
-        LeafNodeIndex(index)
-    }
-
     /// Checks that the wrapped index is valid. Used only for verification
     fn valid(&self) -> bool {
         self.0 < MAX_INDEX
+    }
+}
+
+#[attributes]
+impl LeafNodeIndex {
+    /// Create a new `LeafNodeIndex` from a `u32`.
+    pub fn new(index: u32) -> Self {
+        LeafNodeIndex(index)
     }
 
     /// Return the inner value as `u32`.
@@ -65,6 +68,7 @@ impl LeafNodeIndex {
     }
 
     /// Warning: Only use when the node index represents a leaf node
+    #[requires(node_index % 2 == 0)]
     fn from_tree_index(node_index: u32) -> Self {
         debug_assert!(node_index.is_multiple_of(2));
         LeafNodeIndex(node_index / 2)
@@ -77,14 +81,17 @@ pub struct ParentNodeIndex(u32);
 
 #[attributes]
 impl ParentNodeIndex {
+    /// Checks that the wrapped index is valid. Used only for verification
+    fn valid(&self) -> bool {
+        self.0 < MAX_INDEX - 1
+    }
+}
+
+#[attributes]
+impl ParentNodeIndex {
     /// Create a new `ParentNodeIndex` from a `u32`.
     pub(crate) fn new(index: u32) -> Self {
         ParentNodeIndex(index)
-    }
-
-    /// Checks that the wrapped index is valid. Used only for verification
-    fn valid(&self) -> bool {
-        self.0 < MAX_INDEX
     }
 
     /// Return the inner value as `u32`.
@@ -148,20 +155,23 @@ pub enum TreeNodeIndex {
 
 #[attributes]
 impl TreeNodeIndex {
+    /// Checks that the wrapped index is valid. Used only for verification
+    fn valid(&self) -> bool {
+        match self {
+            TreeNodeIndex::Leaf(leaf_node_index) => leaf_node_index.valid(),
+            TreeNodeIndex::Parent(parent_node_index) => parent_node_index.valid(),
+        }
+    }
+}
+
+#[attributes]
+impl TreeNodeIndex {
     /// Create a new `TreeNodeIndex` from a `u32`.
     fn new(index: u32) -> Self {
         if index.is_multiple_of(2) {
             TreeNodeIndex::Leaf(LeafNodeIndex::from_tree_index(index))
         } else {
             TreeNodeIndex::Parent(ParentNodeIndex::from_tree_index(index))
-        }
-    }
-
-    /// Checks that the wrapped index is valid. Used only for verification
-    fn valid(&self) -> bool {
-        match self {
-            TreeNodeIndex::Leaf(leaf_node_index) => leaf_node_index.valid(),
-            TreeNodeIndex::Parent(parent_node_index) => parent_node_index.valid(),
         }
     }
 
@@ -216,9 +226,19 @@ pub(crate) struct TreeSize(u32);
 
 #[attributes]
 impl TreeSize {
+    /// Checks that the tree size is within bounds. Used only for verification.
+    fn valid(&self) -> bool {
+        MIN_TREE_SIZE <= self.0 && self.0 <= MAX_TREE_SIZE && self.0 % 2 == 1
+    }
+}
+
+#[attributes]
+impl TreeSize {
     /// Create a new `TreeSize` from `nodes`, which will be rounded up to the
     /// next power of 2. The tree size then reflects the smallest tree that can
     /// contain the number of nodes.
+    #[requires(nodes < MAX_TREE_SIZE)]
+    #[ensures(|result| result.valid())]
     pub(crate) fn new(nodes: u32) -> Self {
         let k = log2(nodes);
         TreeSize((1 << (k + 1)) - 1)
@@ -252,7 +272,7 @@ impl TreeSize {
     }
 
     /// Increase the size.
-    #[requires(self.0 < MAX_TREE_SIZE)]
+    #[requires(self.0 < MAX_TREE_SIZE / 2)]
     pub(super) fn inc(&mut self) {
         self.0 = self.0 * 2 + 1;
     }
@@ -326,14 +346,14 @@ pub fn level(index: u32) -> usize {
     k
 }
 
-#[requires({ let s = size.u32(); s > 0 && s <= MAX_TREE_SIZE})]
+#[requires(size.valid())]
 pub(crate) fn root(size: TreeSize) -> TreeNodeIndex {
     let size = size.u32();
     debug_assert!(size > 0);
     TreeNodeIndex::new((1 << log2(size)) - 1)
 }
 
-#[requires(index.u32() < MAX_INDEX)]
+#[requires(index.valid())]
 pub(crate) fn left(index: ParentNodeIndex) -> TreeNodeIndex {
     let x = index.to_tree_index();
     let k = level(x);
@@ -342,7 +362,7 @@ pub(crate) fn left(index: ParentNodeIndex) -> TreeNodeIndex {
     TreeNodeIndex::new(index)
 }
 
-#[requires(index.u32() < MAX_INDEX)]
+#[requires(index.valid())]
 pub(crate) fn right(index: ParentNodeIndex) -> TreeNodeIndex {
     let x = index.to_tree_index();
     let k = level(x);
@@ -353,6 +373,8 @@ pub(crate) fn right(index: ParentNodeIndex) -> TreeNodeIndex {
 
 /// Warning: There is no check about the tree size and whether the parent is
 /// beyond the root
+#[requires(x.valid())]
+#[ensures(|r| r.u32() < MAX_INDEX)] // Cannot be r.valid() (MAX_INDEX - 1)
 fn parent(x: TreeNodeIndex) -> ParentNodeIndex {
     let x = x.u32();
     let k = level(x);
@@ -367,6 +389,8 @@ pub(crate) fn test_parent(index: TreeNodeIndex) -> ParentNodeIndex {
     parent(index)
 }
 
+/// Should not be called on the root
+#[requires(index.valid())]
 fn sibling(index: TreeNodeIndex) -> TreeNodeIndex {
     let p = parent(index);
     match index.u32().cmp(&p.to_tree_index()) {
@@ -384,15 +408,9 @@ pub(crate) fn test_sibling(index: TreeNodeIndex) -> TreeNodeIndex {
 
 /// Direct path from a node to the root.
 /// Does not include the node itself.
-#[requires({
-    let s = size.u32();
-    s > 0 &&
-    s <= MAX_TREE_SIZE &&
-    node_index.u32() < size.leaf_count()})]
+#[requires(size.valid() && node_index.u32() < size.leaf_count())]
 #[ensures(|result|
-    forall(|i: usize| implies(
-        i < result.len(),
-        2 * result[i].u32() + 1 < (1u32 << 31) - 1))
+    forall(|i: usize| implies(i < result.len(), result[i].valid()))
     .and(result.len() <= 30))]
 pub(crate) fn direct_path(node_index: LeafNodeIndex, size: TreeSize) -> Vec<ParentNodeIndex> {
     let r = root(size).u32();
@@ -408,12 +426,7 @@ pub(crate) fn direct_path(node_index: LeafNodeIndex, size: TreeSize) -> Vec<Pare
 }
 
 /// Copath of a leaf node.
-#[requires({
-    let s = size.u32();
-    s > 0 &&
-    s <= MAX_TREE_SIZE &&
-    leaf_index.u32() < size.leaf_count()
-  })]
+#[requires(size.valid() && leaf_index.u32() < size.leaf_count())]
 pub(crate) fn copath(leaf_index: LeafNodeIndex, size: TreeSize) -> Vec<TreeNodeIndex> {
     let mut direct_path = direct_path(leaf_index, size);
     if !direct_path.is_empty() {
@@ -430,7 +443,7 @@ pub(crate) fn copath(leaf_index: LeafNodeIndex, size: TreeSize) -> Vec<TreeNodeI
 
 /// Common ancestor of two leaf nodes, aka the node where their direct paths
 /// intersect.
-#[requires(x.u32() < MAX_INDEX && y.u32() < MAX_INDEX && x.u32() != y.u32())]
+#[requires(x.valid() && y.valid() && x.u32() != y.u32())]
 pub(super) fn lowest_common_ancestor(x: LeafNodeIndex, y: LeafNodeIndex) -> ParentNodeIndex {
     let x = x.to_tree_index();
     let y = y.to_tree_index();
@@ -453,12 +466,7 @@ pub(super) fn lowest_common_ancestor(x: LeafNodeIndex, y: LeafNodeIndex) -> Pare
 
 /// The common direct path of two leaf nodes, i.e. the path from their common
 /// ancestor to the root.
-#[requires({
-    let s = size.u32();
-    s > 0 &&
-    s <= MAX_TREE_SIZE &&
-    x.u32() < size.leaf_count() &&
-    y.u32() < size.leaf_count()})]
+#[requires( size.valid() && x.u32() < size.leaf_count() && y.u32() < size.leaf_count())]
 pub(crate) fn common_direct_path(
     x: LeafNodeIndex,
     y: LeafNodeIndex,
@@ -496,10 +504,7 @@ pub(crate) fn node_width(n: usize) -> usize {
     }
 }
 
-#[requires(match node_index {
-      TreeNodeIndex::Leaf(l) => l.u32() < MAX_INDEX,
-      TreeNodeIndex::Parent(p) => p.u32() < MAX_INDEX,
-  })]
+#[requires(node_index.valid())]
 pub(crate) fn is_node_in_tree(node_index: TreeNodeIndex, size: TreeSize) -> bool {
     node_index.u32() < size.u32()
 }
