openmls/proofs/aeneas-lean/Openmls/Extraction/Funs.lean
@@ -186,27 +186,8 @@ def binary_tree.array_representation.treemath.LeafNodeIndex.Insts.CoreHashHash
     corehashHasherInst
 }
 
-/-- [openmls::binary_tree::array_representation::treemath::_]
-    Source: 'openmls/src/binary_tree/array_representation/treemath.rs', lines 24:4-24:13 -/
-@[global_simps, irreducible]
-def binary_tree.array_representation.treemath._ : Unit := ()
-
-/-- [openmls::binary_tree::array_representation::treemath::_#1]
-    Source: 'openmls/src/binary_tree/array_representation/treemath.rs', lines 25:4-25:15 -/
-@[global_simps, irreducible]
-def binary_tree.array_representation.treemath.__1 : Unit := ()
-
-/-- [openmls::binary_tree::array_representation::treemath::{openmls::binary_tree::array_representation::treemath::LeafNodeIndex}::new]:
-    Source: 'openmls/src/binary_tree/array_representation/treemath.rs', lines 42:4-44:5
-    Visibility: public -/
-def binary_tree.array_representation.treemath.LeafNodeIndex.new
-  (index : Std.U32) :
-  Result binary_tree.array_representation.treemath.LeafNodeIndex
-  := do
-  ok index
-
 /-- [openmls::binary_tree::array_representation::treemath::{openmls::binary_tree::array_representation::treemath::LeafNodeIndex}::valid]:
-    Source: 'openmls/src/binary_tree/array_representation/treemath.rs', lines 47:4-49:5 -/
+    Source: 'openmls/src/binary_tree/array_representation/treemath.rs', lines 42:4-44:5 -/
 def binary_tree.array_representation.treemath.LeafNodeIndex.valid
   (self : binary_tree.array_representation.treemath.LeafNodeIndex) :
   Result Bool
@@ -214,8 +195,17 @@ def binary_tree.array_representation.treemath.LeafNodeIndex.valid
   let i ← binary_tree.array_representation.treemath.MAX_INDEX
   ok (self < i)
 
+/-- [openmls::binary_tree::array_representation::treemath::{openmls::binary_tree::array_representation::treemath::LeafNodeIndex}::new]:
+    Source: 'openmls/src/binary_tree/array_representation/treemath.rs', lines 50:4-52:5
+    Visibility: public -/
+def binary_tree.array_representation.treemath.LeafNodeIndex.new
+  (index : Std.U32) :
+  Result binary_tree.array_representation.treemath.LeafNodeIndex
+  := do
+  ok index
+
 /-- [openmls::binary_tree::array_representation::treemath::{openmls::binary_tree::array_representation::treemath::LeafNodeIndex}::u32]:
-    Source: 'openmls/src/binary_tree/array_representation/treemath.rs', lines 52:4-54:5
+    Source: 'openmls/src/binary_tree/array_representation/treemath.rs', lines 55:4-57:5
     Visibility: public -/
 def binary_tree.array_representation.treemath.LeafNodeIndex.u32
   (self : binary_tree.array_representation.treemath.LeafNodeIndex) :
@@ -224,7 +214,7 @@ def binary_tree.array_representation.treemath.LeafNodeIndex.u32
   ok self
 
 /-- [openmls::binary_tree::array_representation::treemath::{openmls::binary_tree::array_representation::treemath::LeafNodeIndex}::usize]:
-    Source: 'openmls/src/binary_tree/array_representation/treemath.rs', lines 57:4-59:5
+    Source: 'openmls/src/binary_tree/array_representation/treemath.rs', lines 60:4-62:5
     Visibility: public -/
 def binary_tree.array_representation.treemath.LeafNodeIndex.usize
   (self : binary_tree.array_representation.treemath.LeafNodeIndex) :
@@ -234,7 +224,7 @@ def binary_tree.array_representation.treemath.LeafNodeIndex.usize
   ok (UScalar.cast .Usize i)
 
 /-- [openmls::binary_tree::array_representation::treemath::{openmls::binary_tree::array_representation::treemath::LeafNodeIndex}::to_tree_index]:
-    Source: 'openmls/src/binary_tree/array_representation/treemath.rs', lines 63:4-65:5 -/
+    Source: 'openmls/src/binary_tree/array_representation/treemath.rs', lines 66:4-68:5 -/
 def binary_tree.array_representation.treemath.LeafNodeIndex.to_tree_index
   (self : binary_tree.array_representation.treemath.LeafNodeIndex) :
   Result Std.U32
@@ -242,7 +232,7 @@ def binary_tree.array_representation.treemath.LeafNodeIndex.to_tree_index
   self * 2#u32
 
 /-- [openmls::binary_tree::array_representation::treemath::{openmls::binary_tree::array_representation::treemath::LeafNodeIndex}::from_tree_index]:
-    Source: 'openmls/src/binary_tree/array_representation/treemath.rs', lines 68:4-71:5 -/
+    Source: 'openmls/src/binary_tree/array_representation/treemath.rs', lines 72:4-75:5 -/
 def binary_tree.array_representation.treemath.LeafNodeIndex.from_tree_index
   (node_index : Std.U32) :
   Result binary_tree.array_representation.treemath.LeafNodeIndex
@@ -253,7 +243,7 @@ def binary_tree.array_representation.treemath.LeafNodeIndex.from_tree_index
   ok i
 
 /-- [openmls::binary_tree::array_representation::treemath::{impl core::clone::Clone for openmls::binary_tree::array_representation::treemath::ParentNodeIndex}::clone]:
-    Source: 'openmls/src/binary_tree/array_representation/treemath.rs', lines 75:16-75:21
+    Source: 'openmls/src/binary_tree/array_representation/treemath.rs', lines 79:16-79:21
     Visibility: public -/
 def
   binary_tree.array_representation.treemath.ParentNodeIndex.Insts.CoreCloneClone.clone
@@ -263,7 +253,7 @@ def
   ok self
 
 /-- Trait implementation: [openmls::binary_tree::array_representation::treemath::{impl core::clone::Clone for openmls::binary_tree::array_representation::treemath::ParentNodeIndex}]
-    Source: 'openmls/src/binary_tree/array_representation/treemath.rs', lines 75:16-75:21 -/
+    Source: 'openmls/src/binary_tree/array_representation/treemath.rs', lines 79:16-79:21 -/
 @[reducible]
 def
   binary_tree.array_representation.treemath.ParentNodeIndex.Insts.CoreCloneClone
@@ -274,7 +264,7 @@ def
 }
 
 /-- Trait implementation: [openmls::binary_tree::array_representation::treemath::{impl core::marker::Copy for openmls::binary_tree::array_representation::treemath::ParentNodeIndex}]
-    Source: 'openmls/src/binary_tree/array_representation/treemath.rs', lines 75:23-75:27 -/
+    Source: 'openmls/src/binary_tree/array_representation/treemath.rs', lines 79:23-79:27 -/
 @[reducible]
 def
   binary_tree.array_representation.treemath.ParentNodeIndex.Insts.CoreMarkerCopy
@@ -285,7 +275,7 @@ def
 }
 
 /-- Trait implementation: [openmls::binary_tree::array_representation::treemath::{impl core::marker::StructuralPartialEq for openmls::binary_tree::array_representation::treemath::ParentNodeIndex}]
-    Source: 'openmls/src/binary_tree/array_representation/treemath.rs', lines 75:29-75:38 -/
+    Source: 'openmls/src/binary_tree/array_representation/treemath.rs', lines 79:29-79:38 -/
 @[reducible]
 def
   binary_tree.array_representation.treemath.ParentNodeIndex.Insts.CoreMarkerStructuralPartialEq
@@ -294,7 +284,7 @@ def
 }
 
 /-- [openmls::binary_tree::array_representation::treemath::{impl core::cmp::PartialEq<openmls::binary_tree::array_representation::treemath::ParentNodeIndex> for openmls::binary_tree::array_representation::treemath::ParentNodeIndex}::eq]:
-    Source: 'openmls/src/binary_tree/array_representation/treemath.rs', lines 75:29-75:38
+    Source: 'openmls/src/binary_tree/array_representation/treemath.rs', lines 79:29-79:38
     Visibility: public -/
 def
   binary_tree.array_representation.treemath.ParentNodeIndex.Insts.CoreCmpPartialEqParentNodeIndex.eq
@@ -305,7 +295,7 @@ def
   ok (self = other)
 
 /-- Trait implementation: [openmls::binary_tree::array_representation::treemath::{impl core::cmp::PartialEq<openmls::binary_tree::array_representation::treemath::ParentNodeIndex> for openmls::binary_tree::array_representation::treemath::ParentNodeIndex}]
-    Source: 'openmls/src/binary_tree/array_representation/treemath.rs', lines 75:29-75:38 -/
+    Source: 'openmls/src/binary_tree/array_representation/treemath.rs', lines 79:29-79:38 -/
 @[reducible]
 def
   binary_tree.array_representation.treemath.ParentNodeIndex.Insts.CoreCmpPartialEqParentNodeIndex
@@ -317,7 +307,7 @@ def
 }
 
 /-- Trait implementation: [openmls::binary_tree::array_representation::treemath::{impl core::cmp::Eq for openmls::binary_tree::array_representation::treemath::ParentNodeIndex}]
-    Source: 'openmls/src/binary_tree/array_representation/treemath.rs', lines 75:40-75:42 -/
+    Source: 'openmls/src/binary_tree/array_representation/treemath.rs', lines 79:40-79:42 -/
 @[reducible]
 def binary_tree.array_representation.treemath.ParentNodeIndex.Insts.CoreCmpEq :
   core.cmp.Eq binary_tree.array_representation.treemath.ParentNodeIndex := {
@@ -326,7 +316,7 @@ def binary_tree.array_representation.treemath.ParentNodeIndex.Insts.CoreCmpEq :
 }
 
 /-- [openmls::binary_tree::array_representation::treemath::{impl core::cmp::Ord for openmls::binary_tree::array_representation::treemath::ParentNodeIndex}::cmp]:
-    Source: 'openmls/src/binary_tree/array_representation/treemath.rs', lines 75:56-75:59
+    Source: 'openmls/src/binary_tree/array_representation/treemath.rs', lines 79:56-79:59
     Visibility: public -/
 def
   binary_tree.array_representation.treemath.ParentNodeIndex.Insts.CoreCmpOrd.cmp
@@ -337,7 +327,7 @@ def
   core.U32.Insts.CoreCmpOrd.cmp self other
 
 /-- [openmls::binary_tree::array_representation::treemath::{impl core::cmp::PartialOrd<openmls::binary_tree::array_representation::treemath::ParentNodeIndex> for openmls::binary_tree::array_representation::treemath::ParentNodeIndex}::partial_cmp]:
-    Source: 'openmls/src/binary_tree/array_representation/treemath.rs', lines 75:44-75:54
+    Source: 'openmls/src/binary_tree/array_representation/treemath.rs', lines 79:44-79:54
     Visibility: public -/
 def
   binary_tree.array_representation.treemath.ParentNodeIndex.Insts.CoreCmpPartialOrdParentNodeIndex.partial_cmp
@@ -351,7 +341,7 @@ def
   ok (core.option.Option.Some o)
 
 /-- Trait implementation: [openmls::binary_tree::array_representation::treemath::{impl core::cmp::PartialOrd<openmls::binary_tree::array_representation::treemath::ParentNodeIndex> for openmls::binary_tree::array_representation::treemath::ParentNodeIndex}]
-    Source: 'openmls/src/binary_tree/array_representation/treemath.rs', lines 75:44-75:54 -/
+    Source: 'openmls/src/binary_tree/array_representation/treemath.rs', lines 79:44-79:54 -/
 @[reducible]
 def
   binary_tree.array_representation.treemath.ParentNodeIndex.Insts.CoreCmpPartialOrdParentNodeIndex
@@ -365,7 +355,7 @@ def
 }
 
 /-- Trait implementation: [openmls::binary_tree::array_representation::treemath::{impl core::cmp::Ord for openmls::binary_tree::array_representation::treemath::ParentNodeIndex}]
-    Source: 'openmls/src/binary_tree/array_representation/treemath.rs', lines 75:56-75:59 -/
+    Source: 'openmls/src/binary_tree/array_representation/treemath.rs', lines 79:56-79:59 -/
 @[reducible]
 def binary_tree.array_representation.treemath.ParentNodeIndex.Insts.CoreCmpOrd
   : core.cmp.Ord binary_tree.array_representation.treemath.ParentNodeIndex := {
@@ -377,35 +367,26 @@ def binary_tree.array_representation.treemath.ParentNodeIndex.Insts.CoreCmpOrd
     binary_tree.array_representation.treemath.ParentNodeIndex.Insts.CoreCmpOrd.cmp
 }
 
-/-- [openmls::binary_tree::array_representation::treemath::_#2]
-    Source: 'openmls/src/binary_tree/array_representation/treemath.rs', lines 75:61-75:70 -/
-@[global_simps, irreducible]
-def binary_tree.array_representation.treemath.__2 : Unit := ()
-
-/-- [openmls::binary_tree::array_representation::treemath::_#3]
-    Source: 'openmls/src/binary_tree/array_representation/treemath.rs', lines 75:72-75:83 -/
-@[global_simps, irreducible]
-def binary_tree.array_representation.treemath.__3 : Unit := ()
+/-- [openmls::binary_tree::array_representation::treemath::{openmls::binary_tree::array_representation::treemath::ParentNodeIndex}::valid]:
+    Source: 'openmls/src/binary_tree/array_representation/treemath.rs', lines 85:4-87:5 -/
+def binary_tree.array_representation.treemath.ParentNodeIndex.valid
+  (self : binary_tree.array_representation.treemath.ParentNodeIndex) :
+  Result Bool
+  := do
+  let i ← binary_tree.array_representation.treemath.MAX_INDEX
+  let i1 ← i - 1#u32
+  ok (self < i1)
 
 /-- [openmls::binary_tree::array_representation::treemath::{openmls::binary_tree::array_representation::treemath::ParentNodeIndex}::new]:
-    Source: 'openmls/src/binary_tree/array_representation/treemath.rs', lines 81:4-83:5 -/
+    Source: 'openmls/src/binary_tree/array_representation/treemath.rs', lines 93:4-95:5 -/
 def binary_tree.array_representation.treemath.ParentNodeIndex.new
   (index : Std.U32) :
   Result binary_tree.array_representation.treemath.ParentNodeIndex
   := do
   ok index
 
-/-- [openmls::binary_tree::array_representation::treemath::{openmls::binary_tree::array_representation::treemath::ParentNodeIndex}::valid]:
-    Source: 'openmls/src/binary_tree/array_representation/treemath.rs', lines 86:4-88:5 -/
-def binary_tree.array_representation.treemath.ParentNodeIndex.valid
-  (self : binary_tree.array_representation.treemath.ParentNodeIndex) :
-  Result Bool
-  := do
-  let i ← binary_tree.array_representation.treemath.MAX_INDEX
-  ok (self < i)
-
 /-- [openmls::binary_tree::array_representation::treemath::{openmls::binary_tree::array_representation::treemath::ParentNodeIndex}::u32]:
-    Source: 'openmls/src/binary_tree/array_representation/treemath.rs', lines 91:4-93:5
+    Source: 'openmls/src/binary_tree/array_representation/treemath.rs', lines 98:4-100:5
     Visibility: public -/
 def binary_tree.array_representation.treemath.ParentNodeIndex.u32
   (self : binary_tree.array_representation.treemath.ParentNodeIndex) :
@@ -414,7 +395,7 @@ def binary_tree.array_representation.treemath.ParentNodeIndex.u32
   ok self
 
 /-- [openmls::binary_tree::array_representation::treemath::{openmls::binary_tree::array_representation::treemath::ParentNodeIndex}::usize]:
-    Source: 'openmls/src/binary_tree/array_representation/treemath.rs', lines 95:4-97:5 -/
+    Source: 'openmls/src/binary_tree/array_representation/treemath.rs', lines 102:4-104:5 -/
 def binary_tree.array_representation.treemath.ParentNodeIndex.usize
   (self : binary_tree.array_representation.treemath.ParentNodeIndex) :
   Result Std.Usize
@@ -422,7 +403,7 @@ def binary_tree.array_representation.treemath.ParentNodeIndex.usize
   ok (UScalar.cast .Usize self)
 
 /-- [openmls::binary_tree::array_representation::treemath::{openmls::binary_tree::array_representation::treemath::ParentNodeIndex}::to_tree_index]:
-    Source: 'openmls/src/binary_tree/array_representation/treemath.rs', lines 101:4-103:5 -/
+    Source: 'openmls/src/binary_tree/array_representation/treemath.rs', lines 108:4-110:5 -/
 def binary_tree.array_representation.treemath.ParentNodeIndex.to_tree_index
   (self : binary_tree.array_representation.treemath.ParentNodeIndex) :
   Result Std.U32
@@ -431,7 +412,7 @@ def binary_tree.array_representation.treemath.ParentNodeIndex.to_tree_index
   i + 1#u32
 
 /-- [openmls::binary_tree::array_representation::treemath::{openmls::binary_tree::array_representation::treemath::ParentNodeIndex}::from_tree_index]:
-    Source: 'openmls/src/binary_tree/array_representation/treemath.rs', lines 107:4-111:5 -/
+    Source: 'openmls/src/binary_tree/array_representation/treemath.rs', lines 114:4-118:5 -/
 def binary_tree.array_representation.treemath.ParentNodeIndex.from_tree_index
   (node_index : Std.U32) :
   Result binary_tree.array_representation.treemath.ParentNodeIndex
@@ -444,7 +425,7 @@ def binary_tree.array_representation.treemath.ParentNodeIndex.from_tree_index
   ok i2
 
 /-- [openmls::binary_tree::array_representation::treemath::{impl core::convert::From<openmls::binary_tree::array_representation::treemath::LeafNodeIndex> for openmls::binary_tree::array_representation::treemath::TreeNodeIndex}::from]:
-    Source: 'openmls/src/binary_tree/array_representation/treemath.rs', lines 131:4-133:5
+    Source: 'openmls/src/binary_tree/array_representation/treemath.rs', lines 138:4-140:5
     Visibility: public -/
 def
   binary_tree.array_representation.treemath.TreeNodeIndex.Insts.CoreConvertFromLeafNodeIndex.from
@@ -454,7 +435,7 @@ def
   ok (binary_tree.array_representation.treemath.TreeNodeIndex.Leaf leaf_index)
 
 /-- Trait implementation: [openmls::binary_tree::array_representation::treemath::{impl core::convert::From<openmls::binary_tree::array_representation::treemath::LeafNodeIndex> for openmls::binary_tree::array_representation::treemath::TreeNodeIndex}]
-    Source: 'openmls/src/binary_tree/array_representation/treemath.rs', lines 130:0-134:1 -/
+    Source: 'openmls/src/binary_tree/array_representation/treemath.rs', lines 137:0-141:1 -/
 @[reducible]
 def
   binary_tree.array_representation.treemath.TreeNodeIndex.Insts.CoreConvertFromLeafNodeIndex
@@ -465,7 +446,7 @@ def
 }
 
 /-- [openmls::binary_tree::array_representation::treemath::{impl core::convert::From<openmls::binary_tree::array_representation::treemath::ParentNodeIndex> for openmls::binary_tree::array_representation::treemath::TreeNodeIndex}::from]:
-    Source: 'openmls/src/binary_tree/array_representation/treemath.rs', lines 137:4-139:5
+    Source: 'openmls/src/binary_tree/array_representation/treemath.rs', lines 144:4-146:5
     Visibility: public -/
 def
   binary_tree.array_representation.treemath.TreeNodeIndex.Insts.CoreConvertFromParentNodeIndex.from
@@ -476,7 +457,7 @@ def
     parent_index)
 
 /-- Trait implementation: [openmls::binary_tree::array_representation::treemath::{impl core::convert::From<openmls::binary_tree::array_representation::treemath::ParentNodeIndex> for openmls::binary_tree::array_representation::treemath::TreeNodeIndex}]
-    Source: 'openmls/src/binary_tree/array_representation/treemath.rs', lines 136:0-140:1 -/
+    Source: 'openmls/src/binary_tree/array_representation/treemath.rs', lines 143:0-147:1 -/
 @[reducible]
 def
   binary_tree.array_representation.treemath.TreeNodeIndex.Insts.CoreConvertFromParentNodeIndex
@@ -487,7 +468,7 @@ def
 }
 
 /-- [openmls::binary_tree::array_representation::treemath::{impl core::clone::Clone for openmls::binary_tree::array_representation::treemath::TreeNodeIndex}::clone]:
-    Source: 'openmls/src/binary_tree/array_representation/treemath.rs', lines 143:16-143:21
+    Source: 'openmls/src/binary_tree/array_representation/treemath.rs', lines 150:16-150:21
     Visibility: public -/
 def
   binary_tree.array_representation.treemath.TreeNodeIndex.Insts.CoreCloneClone.clone
@@ -497,7 +478,7 @@ def
   ok self
 
 /-- Trait implementation: [openmls::binary_tree::array_representation::treemath::{impl core::clone::Clone for openmls::binary_tree::array_representation::treemath::TreeNodeIndex}]
-    Source: 'openmls/src/binary_tree/array_representation/treemath.rs', lines 143:16-143:21 -/
+    Source: 'openmls/src/binary_tree/array_representation/treemath.rs', lines 150:16-150:21 -/
 @[reducible]
 def
   binary_tree.array_representation.treemath.TreeNodeIndex.Insts.CoreCloneClone
@@ -508,7 +489,7 @@ def
 }
 
 /-- Trait implementation: [openmls::binary_tree::array_representation::treemath::{impl core::marker::Copy for openmls::binary_tree::array_representation::treemath::TreeNodeIndex}]
-    Source: 'openmls/src/binary_tree/array_representation/treemath.rs', lines 143:23-143:27 -/
+    Source: 'openmls/src/binary_tree/array_representation/treemath.rs', lines 150:23-150:27 -/
 @[reducible]
 def
   binary_tree.array_representation.treemath.TreeNodeIndex.Insts.CoreMarkerCopy
@@ -519,7 +500,7 @@ def
 }
 
 /-- Trait implementation: [openmls::binary_tree::array_representation::treemath::{impl core::marker::StructuralPartialEq for openmls::binary_tree::array_representation::treemath::TreeNodeIndex}]
-    Source: 'openmls/src/binary_tree/array_representation/treemath.rs', lines 143:29-143:38 -/
+    Source: 'openmls/src/binary_tree/array_representation/treemath.rs', lines 150:29-150:38 -/
 @[reducible]
 def
   binary_tree.array_representation.treemath.TreeNodeIndex.Insts.CoreMarkerStructuralPartialEq
@@ -528,7 +509,7 @@ def
 }
 
 /-- [openmls::binary_tree::array_representation::treemath::{impl core::cmp::PartialEq<openmls::binary_tree::array_representation::treemath::TreeNodeIndex> for openmls::binary_tree::array_representation::treemath::TreeNodeIndex}::eq]:
-    Source: 'openmls/src/binary_tree/array_representation/treemath.rs', lines 143:29-143:38
+    Source: 'openmls/src/binary_tree/array_representation/treemath.rs', lines 150:29-150:38
     Visibility: public -/
 def
   binary_tree.array_representation.treemath.TreeNodeIndex.Insts.CoreCmpPartialEqTreeNodeIndex.eq
@@ -561,7 +542,7 @@ def
   else ok false
 
 /-- Trait implementation: [openmls::binary_tree::array_representation::treemath::{impl core::cmp::PartialEq<openmls::binary_tree::array_representation::treemath::TreeNodeIndex> for openmls::binary_tree::array_representation::treemath::TreeNodeIndex}]
-    Source: 'openmls/src/binary_tree/array_representation/treemath.rs', lines 143:29-143:38 -/
+    Source: 'openmls/src/binary_tree/array_representation/treemath.rs', lines 150:29-150:38 -/
 @[reducible]
 def
   binary_tree.array_representation.treemath.TreeNodeIndex.Insts.CoreCmpPartialEqTreeNodeIndex
@@ -572,7 +553,7 @@ def
 }
 
 /-- Trait implementation: [openmls::binary_tree::array_representation::treemath::{impl core::cmp::Eq for openmls::binary_tree::array_representation::treemath::TreeNodeIndex}]
-    Source: 'openmls/src/binary_tree/array_representation/treemath.rs', lines 143:40-143:42 -/
+    Source: 'openmls/src/binary_tree/array_representation/treemath.rs', lines 150:40-150:42 -/
 @[reducible]
 def binary_tree.array_representation.treemath.TreeNodeIndex.Insts.CoreCmpEq :
   core.cmp.Eq binary_tree.array_representation.treemath.TreeNodeIndex := {
@@ -580,18 +561,24 @@ def binary_tree.array_representation.treemath.TreeNodeIndex.Insts.CoreCmpEq :
     binary_tree.array_representation.treemath.TreeNodeIndex.Insts.CoreCmpPartialEqTreeNodeIndex
 }
 
-/-- [openmls::binary_tree::array_representation::treemath::_#4]
-    Source: 'openmls/src/binary_tree/array_representation/treemath.rs', lines 143:44-143:53 -/
-@[global_simps, irreducible]
-def binary_tree.array_representation.treemath.__4 : Unit := ()
-
-/-- [openmls::binary_tree::array_representation::treemath::_#5]
-    Source: 'openmls/src/binary_tree/array_representation/treemath.rs', lines 143:55-143:66 -/
-@[global_simps, irreducible]
-def binary_tree.array_representation.treemath.__5 : Unit := ()
+/-- [openmls::binary_tree::array_representation::treemath::{openmls::binary_tree::array_representation::treemath::TreeNodeIndex}::valid]:
+    Source: 'openmls/src/binary_tree/array_representation/treemath.rs', lines 159:4-164:5 -/
+def binary_tree.array_representation.treemath.TreeNodeIndex.valid
+  (self : binary_tree.array_representation.treemath.TreeNodeIndex) :
+  Result Bool
+  := do
+  match self with
+  | binary_tree.array_representation.treemath.TreeNodeIndex.Leaf
+    leaf_node_index =>
+    binary_tree.array_representation.treemath.LeafNodeIndex.valid
+      leaf_node_index
+  | binary_tree.array_representation.treemath.TreeNodeIndex.Parent
+    parent_node_index =>
+    binary_tree.array_representation.treemath.ParentNodeIndex.valid
+      parent_node_index
 
 /-- [openmls::binary_tree::array_representation::treemath::{openmls::binary_tree::array_representation::treemath::TreeNodeIndex}::new]:
-    Source: 'openmls/src/binary_tree/array_representation/treemath.rs', lines 152:4-158:5 -/
+    Source: 'openmls/src/binary_tree/array_representation/treemath.rs', lines 170:4-176:5 -/
 def binary_tree.array_representation.treemath.TreeNodeIndex.new
   (index : Std.U32) :
   Result binary_tree.array_representation.treemath.TreeNodeIndex
@@ -609,24 +596,8 @@ def binary_tree.array_representation.treemath.TreeNodeIndex.new
         index
     ok (binary_tree.array_representation.treemath.TreeNodeIndex.Parent pni)
 
-/-- [openmls::binary_tree::array_representation::treemath::{openmls::binary_tree::array_representation::treemath::TreeNodeIndex}::valid]:
-    Source: 'openmls/src/binary_tree/array_representation/treemath.rs', lines 161:4-166:5 -/
-def binary_tree.array_representation.treemath.TreeNodeIndex.valid
-  (self : binary_tree.array_representation.treemath.TreeNodeIndex) :
-  Result Bool
-  := do
-  match self with
-  | binary_tree.array_representation.treemath.TreeNodeIndex.Leaf
-    leaf_node_index =>
-    binary_tree.array_representation.treemath.LeafNodeIndex.valid
-      leaf_node_index
-  | binary_tree.array_representation.treemath.TreeNodeIndex.Parent
-    parent_node_index =>
-    binary_tree.array_representation.treemath.ParentNodeIndex.valid
-      parent_node_index
-
 /-- [openmls::binary_tree::array_representation::treemath::{openmls::binary_tree::array_representation::treemath::TreeNodeIndex}::u32]:
-    Source: 'openmls/src/binary_tree/array_representation/treemath.rs', lines 176:4-181:5 -/
+    Source: 'openmls/src/binary_tree/array_representation/treemath.rs', lines 186:4-191:5 -/
 def binary_tree.array_representation.treemath.TreeNodeIndex.u32
   (self : binary_tree.array_representation.treemath.TreeNodeIndex) :
   Result Std.U32
@@ -639,7 +610,7 @@ def binary_tree.array_representation.treemath.TreeNodeIndex.u32
       index
 
 /-- [openmls::binary_tree::array_representation::treemath::{impl core::cmp::Ord for openmls::binary_tree::array_representation::treemath::TreeNodeIndex}::cmp]:
-    Source: 'openmls/src/binary_tree/array_representation/treemath.rs', lines 203:4-205:5
+    Source: 'openmls/src/binary_tree/array_representation/treemath.rs', lines 213:4-215:5
     Visibility: public -/
 def
   binary_tree.array_representation.treemath.TreeNodeIndex.Insts.CoreCmpOrd.cmp
@@ -652,7 +623,7 @@ def
   core.U32.Insts.CoreCmpOrd.cmp i i1
 
 /-- [openmls::binary_tree::array_representation::treemath::{impl core::cmp::PartialOrd<openmls::binary_tree::array_representation::treemath::TreeNodeIndex> for openmls::binary_tree::array_representation::treemath::TreeNodeIndex}::partial_cmp]:
-    Source: 'openmls/src/binary_tree/array_representation/treemath.rs', lines 209:4-211:5
+    Source: 'openmls/src/binary_tree/array_representation/treemath.rs', lines 219:4-221:5
     Visibility: public -/
 def
   binary_tree.array_representation.treemath.TreeNodeIndex.Insts.CoreCmpPartialOrdTreeNodeIndex.partial_cmp
@@ -666,7 +637,7 @@ def
   ok (core.option.Option.Some o)
 
 /-- Trait implementation: [openmls::binary_tree::array_representation::treemath::{impl core::cmp::PartialOrd<openmls::binary_tree::array_representation::treemath::TreeNodeIndex> for openmls::binary_tree::array_representation::treemath::TreeNodeIndex}]
-    Source: 'openmls/src/binary_tree/array_representation/treemath.rs', lines 208:0-212:1 -/
+    Source: 'openmls/src/binary_tree/array_representation/treemath.rs', lines 218:0-222:1 -/
 @[reducible]
 def
   binary_tree.array_representation.treemath.TreeNodeIndex.Insts.CoreCmpPartialOrdTreeNodeIndex
@@ -679,7 +650,7 @@ def
 }
 
 /-- Trait implementation: [openmls::binary_tree::array_representation::treemath::{impl core::cmp::Ord for openmls::binary_tree::array_representation::treemath::TreeNodeIndex}]
-    Source: 'openmls/src/binary_tree/array_representation/treemath.rs', lines 202:0-206:1 -/
+    Source: 'openmls/src/binary_tree/array_representation/treemath.rs', lines 212:0-216:1 -/
 @[reducible]
 def binary_tree.array_representation.treemath.TreeNodeIndex.Insts.CoreCmpOrd :
   core.cmp.Ord binary_tree.array_representation.treemath.TreeNodeIndex := {
@@ -692,7 +663,7 @@ def binary_tree.array_representation.treemath.TreeNodeIndex.Insts.CoreCmpOrd :
 }
 
 /-- [openmls::binary_tree::array_representation::treemath::{impl core::clone::Clone for openmls::binary_tree::array_representation::treemath::TreeSize}::clone]:
-    Source: 'openmls/src/binary_tree/array_representation/treemath.rs', lines 214:16-214:21
+    Source: 'openmls/src/binary_tree/array_representation/treemath.rs', lines 224:16-224:21
     Visibility: public -/
 def
   binary_tree.array_representation.treemath.TreeSize.Insts.CoreCloneClone.clone
@@ -702,7 +673,7 @@ def
   ok self
 
 /-- Trait implementation: [openmls::binary_tree::array_representation::treemath::{impl core::clone::Clone for openmls::binary_tree::array_representation::treemath::TreeSize}]
-    Source: 'openmls/src/binary_tree/array_representation/treemath.rs', lines 214:16-214:21 -/
+    Source: 'openmls/src/binary_tree/array_representation/treemath.rs', lines 224:16-224:21 -/
 @[reducible]
 def binary_tree.array_representation.treemath.TreeSize.Insts.CoreCloneClone :
   core.clone.Clone binary_tree.array_representation.treemath.TreeSize := {
@@ -711,7 +682,7 @@ def binary_tree.array_representation.treemath.TreeSize.Insts.CoreCloneClone :
 }
 
 /-- Trait implementation: [openmls::binary_tree::array_representation::treemath::{impl core::marker::Copy for openmls::binary_tree::array_representation::treemath::TreeSize}]
-    Source: 'openmls/src/binary_tree/array_representation/treemath.rs', lines 214:23-214:27 -/
+    Source: 'openmls/src/binary_tree/array_representation/treemath.rs', lines 224:23-224:27 -/
 @[reducible]
 def binary_tree.array_representation.treemath.TreeSize.Insts.CoreMarkerCopy :
   core.marker.Copy binary_tree.array_representation.treemath.TreeSize := {
@@ -720,7 +691,7 @@ def binary_tree.array_representation.treemath.TreeSize.Insts.CoreMarkerCopy :
 }
 
 /-- Trait implementation: [openmls::binary_tree::array_representation::treemath::{impl core::marker::StructuralPartialEq for openmls::binary_tree::array_representation::treemath::TreeSize}]
-    Source: 'openmls/src/binary_tree/array_representation/treemath.rs', lines 214:29-214:38 -/
+    Source: 'openmls/src/binary_tree/array_representation/treemath.rs', lines 224:29-224:38 -/
 @[reducible]
 def
   binary_tree.array_representation.treemath.TreeSize.Insts.CoreMarkerStructuralPartialEq
@@ -729,7 +700,7 @@ def
 }
 
 /-- [openmls::binary_tree::array_representation::treemath::{impl core::cmp::PartialEq<openmls::binary_tree::array_representation::treemath::TreeSize> for openmls::binary_tree::array_representation::treemath::TreeSize}::eq]:
-    Source: 'openmls/src/binary_tree/array_representation/treemath.rs', lines 214:29-214:38
+    Source: 'openmls/src/binary_tree/array_representation/treemath.rs', lines 224:29-224:38
     Visibility: public -/
 def
   binary_tree.array_representation.treemath.TreeSize.Insts.CoreCmpPartialEqTreeSize.eq
@@ -740,7 +711,7 @@ def
   ok (self = other)
 
 /-- Trait implementation: [openmls::binary_tree::array_representation::treemath::{impl core::cmp::PartialEq<openmls::binary_tree::array_representation::treemath::TreeSize> for openmls::binary_tree::array_representation::treemath::TreeSize}]
-    Source: 'openmls/src/binary_tree/array_representation/treemath.rs', lines 214:29-214:38 -/
+    Source: 'openmls/src/binary_tree/array_representation/treemath.rs', lines 224:29-224:38 -/
 @[reducible]
 def
   binary_tree.array_representation.treemath.TreeSize.Insts.CoreCmpPartialEqTreeSize
@@ -751,7 +722,7 @@ def
 }
 
 /-- Trait implementation: [openmls::binary_tree::array_representation::treemath::{impl core::cmp::Eq for openmls::binary_tree::array_representation::treemath::TreeSize}]
-    Source: 'openmls/src/binary_tree/array_representation/treemath.rs', lines 214:40-214:42 -/
+    Source: 'openmls/src/binary_tree/array_representation/treemath.rs', lines 224:40-224:42 -/
 @[reducible]
 def binary_tree.array_representation.treemath.TreeSize.Insts.CoreCmpEq :
   core.cmp.Eq binary_tree.array_representation.treemath.TreeSize := {
@@ -760,7 +731,7 @@ def binary_tree.array_representation.treemath.TreeSize.Insts.CoreCmpEq :
 }
 
 /-- [openmls::binary_tree::array_representation::treemath::{impl core::cmp::Ord for openmls::binary_tree::array_representation::treemath::TreeSize}::cmp]:
-    Source: 'openmls/src/binary_tree/array_representation/treemath.rs', lines 214:56-214:59
+    Source: 'openmls/src/binary_tree/array_representation/treemath.rs', lines 224:56-224:59
     Visibility: public -/
 def binary_tree.array_representation.treemath.TreeSize.Insts.CoreCmpOrd.cmp
   (self : binary_tree.array_representation.treemath.TreeSize)
@@ -770,7 +741,7 @@ def binary_tree.array_representation.treemath.TreeSize.Insts.CoreCmpOrd.cmp
   core.U32.Insts.CoreCmpOrd.cmp self other
 
 /-- [openmls::binary_tree::array_representation::treemath::{impl core::cmp::PartialOrd<openmls::binary_tree::array_representation::treemath::TreeSize> for openmls::binary_tree::array_representation::treemath::TreeSize}::partial_cmp]:
-    Source: 'openmls/src/binary_tree/array_representation/treemath.rs', lines 214:44-214:54
+    Source: 'openmls/src/binary_tree/array_representation/treemath.rs', lines 224:44-224:54
     Visibility: public -/
 def
   binary_tree.array_representation.treemath.TreeSize.Insts.CoreCmpPartialOrdTreeSize.partial_cmp
@@ -784,7 +755,7 @@ def
   ok (core.option.Option.Some o)
 
 /-- Trait implementation: [openmls::binary_tree::array_representation::treemath::{impl core::cmp::PartialOrd<openmls::binary_tree::array_representation::treemath::TreeSize> for openmls::binary_tree::array_representation::treemath::TreeSize}]
-    Source: 'openmls/src/binary_tree/array_representation/treemath.rs', lines 214:44-214:54 -/
+    Source: 'openmls/src/binary_tree/array_representation/treemath.rs', lines 224:44-224:54 -/
 @[reducible]
 def
   binary_tree.array_representation.treemath.TreeSize.Insts.CoreCmpPartialOrdTreeSize
@@ -797,7 +768,7 @@ def
 }
 
 /-- Trait implementation: [openmls::binary_tree::array_representation::treemath::{impl core::cmp::Ord for openmls::binary_tree::array_representation::treemath::TreeSize}]
-    Source: 'openmls/src/binary_tree/array_representation/treemath.rs', lines 214:56-214:59 -/
+    Source: 'openmls/src/binary_tree/array_representation/treemath.rs', lines 224:56-224:59 -/
 @[reducible]
 def binary_tree.array_representation.treemath.TreeSize.Insts.CoreCmpOrd :
   core.cmp.Ord binary_tree.array_representation.treemath.TreeSize := {
@@ -808,18 +779,23 @@ def binary_tree.array_representation.treemath.TreeSize.Insts.CoreCmpOrd :
     binary_tree.array_representation.treemath.TreeSize.Insts.CoreCmpOrd.cmp
 }
 
-/-- [openmls::binary_tree::array_representation::treemath::_#6]
-    Source: 'openmls/src/binary_tree/array_representation/treemath.rs', lines 214:61-214:70 -/
-@[global_simps, irreducible]
-def binary_tree.array_representation.treemath.__6 : Unit := ()
-
-/-- [openmls::binary_tree::array_representation::treemath::_#7]
-    Source: 'openmls/src/binary_tree/array_representation/treemath.rs', lines 214:72-214:83 -/
-@[global_simps, irreducible]
-def binary_tree.array_representation.treemath.__7 : Unit := ()
+/-- [openmls::binary_tree::array_representation::treemath::{openmls::binary_tree::array_representation::treemath::TreeSize}::valid]:
+    Source: 'openmls/src/binary_tree/array_representation/treemath.rs', lines 230:4-232:5 -/
+def binary_tree.array_representation.treemath.TreeSize.valid
+  (self : binary_tree.array_representation.treemath.TreeSize) :
+  Result Bool
+  := do
+  if binary_tree.array_representation.treemath.MIN_TREE_SIZE <= self
+  then
+    let i ← binary_tree.array_representation.treemath.MAX_TREE_SIZE
+    if self <= i
+    then let i1 ← self % 2#u32
+         ok (i1 = 1#u32)
+    else ok false
+  else ok false
 
 /-- [openmls::binary_tree::array_representation::treemath::log2]:
-    Source: 'openmls/src/binary_tree/array_representation/treemath.rs', lines 308:0-313:1 -/
+    Source: 'openmls/src/binary_tree/array_representation/treemath.rs', lines 328:0-333:1 -/
 def binary_tree.array_representation.treemath.log2
   (x : Std.U32) : Result Std.Usize := do
   if x = 0#u32
@@ -830,7 +806,7 @@ def binary_tree.array_representation.treemath.log2
     ok (UScalar.cast .Usize i1)
 
 /-- [openmls::binary_tree::array_representation::treemath::{openmls::binary_tree::array_representation::treemath::TreeSize}::new]:
-    Source: 'openmls/src/binary_tree/array_representation/treemath.rs', lines 222:4-225:5 -/
+    Source: 'openmls/src/binary_tree/array_representation/treemath.rs', lines 242:4-245:5 -/
 def binary_tree.array_representation.treemath.TreeSize.new
   (nodes : Std.U32) :
   Result binary_tree.array_representation.treemath.TreeSize
@@ -842,7 +818,7 @@ def binary_tree.array_representation.treemath.TreeSize.new
   ok i2
 
 /-- [openmls::binary_tree::array_representation::treemath::{openmls::binary_tree::array_representation::treemath::TreeSize}::leaf_count]:
-    Source: 'openmls/src/binary_tree/array_representation/treemath.rs', lines 234:4-236:5 -/
+    Source: 'openmls/src/binary_tree/array_representation/treemath.rs', lines 254:4-256:5 -/
 def binary_tree.array_representation.treemath.TreeSize.leaf_count
   (self : binary_tree.array_representation.treemath.TreeSize) :
   Result Std.U32
@@ -851,7 +827,7 @@ def binary_tree.array_representation.treemath.TreeSize.leaf_count
   i + 1#u32
 
 /-- [openmls::binary_tree::array_representation::treemath::{openmls::binary_tree::array_representation::treemath::TreeSize}::parent_count]:
-    Source: 'openmls/src/binary_tree/array_representation/treemath.rs', lines 239:4-241:5 -/
+    Source: 'openmls/src/binary_tree/array_representation/treemath.rs', lines 259:4-261:5 -/
 def binary_tree.array_representation.treemath.TreeSize.parent_count
   (self : binary_tree.array_representation.treemath.TreeSize) :
   Result Std.U32
@@ -859,7 +835,7 @@ def binary_tree.array_representation.treemath.TreeSize.parent_count
   self / 2#u32
 
 /-- [openmls::binary_tree::array_representation::treemath::{openmls::binary_tree::array_representation::treemath::TreeSize}::u32]:
-    Source: 'openmls/src/binary_tree/array_representation/treemath.rs', lines 244:4-246:5 -/
+    Source: 'openmls/src/binary_tree/array_representation/treemath.rs', lines 264:4-266:5 -/
 def binary_tree.array_representation.treemath.TreeSize.u32
   (self : binary_tree.array_representation.treemath.TreeSize) :
   Result Std.U32
@@ -867,7 +843,7 @@ def binary_tree.array_representation.treemath.TreeSize.u32
   ok self
 
 /-- [openmls::binary_tree::array_representation::treemath::{openmls::binary_tree::array_representation::treemath::TreeSize}::leaf_is_left]:
-    Source: 'openmls/src/binary_tree/array_representation/treemath.rs', lines 250:4-252:5 -/
+    Source: 'openmls/src/binary_tree/array_representation/treemath.rs', lines 270:4-272:5 -/
 def binary_tree.array_representation.treemath.TreeSize.leaf_is_left
   (self : binary_tree.array_representation.treemath.TreeSize)
   (leaf_index : binary_tree.array_representation.treemath.LeafNodeIndex) :
@@ -880,7 +856,7 @@ def binary_tree.array_representation.treemath.TreeSize.leaf_is_left
   ok (i < i2)
 
 /-- [openmls::binary_tree::array_representation::treemath::{openmls::binary_tree::array_representation::treemath::TreeSize}::inc]:
-    Source: 'openmls/src/binary_tree/array_representation/treemath.rs', lines 256:4-258:5 -/
+    Source: 'openmls/src/binary_tree/array_representation/treemath.rs', lines 276:4-278:5 -/
 def binary_tree.array_representation.treemath.TreeSize.inc
   (self : binary_tree.array_representation.treemath.TreeSize) :
   Result binary_tree.array_representation.treemath.TreeSize
@@ -890,7 +866,7 @@ def binary_tree.array_representation.treemath.TreeSize.inc
   ok i1
 
 /-- [openmls::binary_tree::array_representation::treemath::{openmls::binary_tree::array_representation::treemath::TreeSize}::dec]:
-    Source: 'openmls/src/binary_tree/array_representation/treemath.rs', lines 262:4-269:5 -/
+    Source: 'openmls/src/binary_tree/array_representation/treemath.rs', lines 282:4-289:5 -/
 def binary_tree.array_representation.treemath.TreeSize.dec
   (self : binary_tree.array_representation.treemath.TreeSize) :
   Result binary_tree.array_representation.treemath.TreeSize
@@ -903,7 +879,7 @@ def binary_tree.array_representation.treemath.TreeSize.dec
   else ok 0#u32
 
 /-- [openmls::binary_tree::array_representation::treemath::level]: loop body 0:
-    Source: 'openmls/src/binary_tree/array_representation/treemath.rs', lines 323:4-325:5
+    Source: 'openmls/src/binary_tree/array_representation/treemath.rs', lines 343:4-345:5
     Visibility: public -/
 @[rust_loop_body]
 def binary_tree.array_representation.treemath.level_loop.body
@@ -918,7 +894,7 @@ def binary_tree.array_representation.treemath.level_loop.body
   else ok (done k)
 
 /-- [openmls::binary_tree::array_representation::treemath::level]: loop 0:
-    Source: 'openmls/src/binary_tree/array_representation/treemath.rs', lines 323:4-325:5
+    Source: 'openmls/src/binary_tree/array_representation/treemath.rs', lines 343:4-345:5
     Visibility: public -/
 @[rust_loop]
 def binary_tree.array_representation.treemath.level_loop
@@ -929,7 +905,7 @@ def binary_tree.array_representation.treemath.level_loop
     k
 
 /-- [openmls::binary_tree::array_representation::treemath::level]:
-    Source: 'openmls/src/binary_tree/array_representation/treemath.rs', lines 317:0-327:1
+    Source: 'openmls/src/binary_tree/array_representation/treemath.rs', lines 337:0-347:1
     Visibility: public -/
 def binary_tree.array_representation.treemath.level
   (index : Std.U32) : Result Std.Usize := do
@@ -939,7 +915,7 @@ def binary_tree.array_representation.treemath.level
   else binary_tree.array_representation.treemath.level_loop index 0#usize
 
 /-- [openmls::binary_tree::array_representation::treemath::root]:
-    Source: 'openmls/src/binary_tree/array_representation/treemath.rs', lines 330:0-334:1 -/
+    Source: 'openmls/src/binary_tree/array_representation/treemath.rs', lines 350:0-354:1 -/
 def binary_tree.array_representation.treemath.root
   (size : binary_tree.array_representation.treemath.TreeSize) :
   Result binary_tree.array_representation.treemath.TreeNodeIndex
@@ -952,7 +928,7 @@ def binary_tree.array_representation.treemath.root
   binary_tree.array_representation.treemath.TreeNodeIndex.new i2
 
 /-- [openmls::binary_tree::array_representation::treemath::left]:
-    Source: 'openmls/src/binary_tree/array_representation/treemath.rs', lines 337:0-343:1 -/
+    Source: 'openmls/src/binary_tree/array_representation/treemath.rs', lines 357:0-363:1 -/
 def binary_tree.array_representation.treemath.left
   (index : binary_tree.array_representation.treemath.ParentNodeIndex) :
   Result binary_tree.array_representation.treemath.TreeNodeIndex
@@ -968,7 +944,7 @@ def binary_tree.array_representation.treemath.left
   binary_tree.array_representation.treemath.TreeNodeIndex.new index1
 
 /-- [openmls::binary_tree::array_representation::treemath::right]:
-    Source: 'openmls/src/binary_tree/array_representation/treemath.rs', lines 346:0-352:1 -/
+    Source: 'openmls/src/binary_tree/array_representation/treemath.rs', lines 366:0-372:1 -/
 def binary_tree.array_representation.treemath.right
   (index : binary_tree.array_representation.treemath.ParentNodeIndex) :
   Result binary_tree.array_representation.treemath.TreeNodeIndex
@@ -984,7 +960,7 @@ def binary_tree.array_representation.treemath.right
   binary_tree.array_representation.treemath.TreeNodeIndex.new index1
 
 /-- [openmls::binary_tree::array_representation::treemath::parent]:
-    Source: 'openmls/src/binary_tree/array_representation/treemath.rs', lines 356:0-362:1 -/
+    Source: 'openmls/src/binary_tree/array_representation/treemath.rs', lines 378:0-384:1 -/
 def binary_tree.array_representation.treemath.parent
   (x : binary_tree.array_representation.treemath.TreeNodeIndex) :
   Result binary_tree.array_representation.treemath.ParentNodeIndex
@@ -1002,7 +978,7 @@ def binary_tree.array_representation.treemath.parent
     index
 
 /-- [openmls::binary_tree::array_representation::treemath::sibling]:
-    Source: 'openmls/src/binary_tree/array_representation/treemath.rs', lines 370:0-377:1 -/
+    Source: 'openmls/src/binary_tree/array_representation/treemath.rs', lines 394:0-401:1 -/
 def binary_tree.array_representation.treemath.sibling
   (index : binary_tree.array_representation.treemath.TreeNodeIndex) :
   Result binary_tree.array_representation.treemath.TreeNodeIndex
@@ -1018,95 +994,8 @@ def binary_tree.array_representation.treemath.sibling
   | core.cmp.Ordering.Greater =>
     binary_tree.array_representation.treemath.left p
 
-/-- [openmls::binary_tree::array_representation::treemath::_#14::ensures::{impl core::ops::function::Fn<(usize,), hax_lib::prop::Prop> for openmls::binary_tree::array_representation::treemath::_#14::ensures::closure<'_0>}::call]:
-    Source: 'openmls/src/binary_tree/array_representation/treemath.rs', lines 393:11-395:51 -/
-def
-  binary_tree.array_representation.treemath.__14.ensures.closure.Insts.CoreOpsFunctionFnTupleUsizeProp.call
-  (c : binary_tree.array_representation.treemath.__14.ensures.closure)
-  (tupled_args : Std.Usize) :
-  Result Prop
-  := do
-  let i ← alloc.vec.Vec.len c
-  let pni ←
-    alloc.vec.Vec.Insts.CoreOpsIndexIndex.index
-      (core.Usize.Insts.CoreSliceIndexSliceIndexSliceT
-      binary_tree.array_representation.treemath.ParentNodeIndex) c tupled_args
-  let i1 ← binary_tree.array_representation.treemath.ParentNodeIndex.u32 pni
-  let i2 ← 2#u32 * i1
-  let i3 ← i2 + 1#u32
-  let i4 ← 1#u32 <<< 31#i32
-  let i5 ← i4 - 1#u32;
-  pure <| (tupled_args < i) → (i3 < i5)
-
-/-- [openmls::binary_tree::array_representation::treemath::_#14::ensures::{impl core::ops::function::FnMut<(usize,), hax_lib::prop::Prop> for openmls::binary_tree::array_representation::treemath::_#14::ensures::closure<'_0>}::call_mut]:
-    Source: 'openmls/src/binary_tree/array_representation/treemath.rs', lines 393:11-395:51 -/
-def
-  binary_tree.array_representation.treemath.__14.ensures.closure.Insts.CoreOpsFunctionFnMutTupleUsizeProp.call_mut
-  (state : binary_tree.array_representation.treemath.__14.ensures.closure)
-  (args : Std.Usize) :
-  Result (Prop ×
-    binary_tree.array_representation.treemath.__14.ensures.closure)
-  := do
-  let p ←
-    binary_tree.array_representation.treemath.__14.ensures.closure.Insts.CoreOpsFunctionFnTupleUsizeProp.call
-      state args
-  ok (p, state)
-
-/-- [openmls::binary_tree::array_representation::treemath::_#14::ensures::{impl core::ops::function::FnOnce<(usize,), hax_lib::prop::Prop> for openmls::binary_tree::array_representation::treemath::_#14::ensures::closure<'_0>}::call_once]:
-    Source: 'openmls/src/binary_tree/array_representation/treemath.rs', lines 393:11-395:51 -/
-def
-  binary_tree.array_representation.treemath.__14.ensures.closure.Insts.CoreOpsFunctionFnOnceTupleUsizeProp.call_once
-  (c : binary_tree.array_representation.treemath.__14.ensures.closure)
-  (i : Std.Usize) :
-  Result Prop
-  := do
-  let (p, _) ←
-    binary_tree.array_representation.treemath.__14.ensures.closure.Insts.CoreOpsFunctionFnMutTupleUsizeProp.call_mut
-      c i
-  ok p
-
-/-- Trait implementation: [openmls::binary_tree::array_representation::treemath::_#14::ensures::{impl core::ops::function::FnOnce<(usize,), hax_lib::prop::Prop> for openmls::binary_tree::array_representation::treemath::_#14::ensures::closure<'_0>}]
-    Source: 'openmls/src/binary_tree/array_representation/treemath.rs', lines 393:11-395:51 -/
-@[reducible]
-def
-  binary_tree.array_representation.treemath.__14.ensures.closure.Insts.CoreOpsFunctionFnOnceTupleUsizeProp
-  : core.ops.function.FnOnce
-  binary_tree.array_representation.treemath.__14.ensures.closure Std.Usize
-  Prop := {
-  call_once :=
-    binary_tree.array_representation.treemath.__14.ensures.closure.Insts.CoreOpsFunctionFnOnceTupleUsizeProp.call_once
-}
-
-/-- Trait implementation: [openmls::binary_tree::array_representation::treemath::_#14::ensures::{impl core::ops::function::FnMut<(usize,), hax_lib::prop::Prop> for openmls::binary_tree::array_representation::treemath::_#14::ensures::closure<'_0>}]
-    Source: 'openmls/src/binary_tree/array_representation/treemath.rs', lines 393:11-395:51 -/
-@[reducible]
-def
-  binary_tree.array_representation.treemath.__14.ensures.closure.Insts.CoreOpsFunctionFnMutTupleUsizeProp
-  : core.ops.function.FnMut
-  binary_tree.array_representation.treemath.__14.ensures.closure Std.Usize
-  Prop := {
-  FnOnceInst :=
-    binary_tree.array_representation.treemath.__14.ensures.closure.Insts.CoreOpsFunctionFnOnceTupleUsizeProp
-  call_mut :=
-    binary_tree.array_representation.treemath.__14.ensures.closure.Insts.CoreOpsFunctionFnMutTupleUsizeProp.call_mut
-}
-
-/-- Trait implementation: [openmls::binary_tree::array_representation::treemath::_#14::ensures::{impl core::ops::function::Fn<(usize,), hax_lib::prop::Prop> for openmls::binary_tree::array_representation::treemath::_#14::ensures::closure<'_0>}]
-    Source: 'openmls/src/binary_tree/array_representation/treemath.rs', lines 393:11-395:51 -/
-@[reducible]
-def
-  binary_tree.array_representation.treemath.__14.ensures.closure.Insts.CoreOpsFunctionFnTupleUsizeProp
-  : core.ops.function.Fn
-  binary_tree.array_representation.treemath.__14.ensures.closure Std.Usize
-  Prop := {
-  FnMutInst :=
-    binary_tree.array_representation.treemath.__14.ensures.closure.Insts.CoreOpsFunctionFnMutTupleUsizeProp
-  call :=
-    binary_tree.array_representation.treemath.__14.ensures.closure.Insts.CoreOpsFunctionFnTupleUsizeProp.call
-}
-
 /-- [openmls::binary_tree::array_representation::treemath::direct_path]: loop body 0:
-    Source: 'openmls/src/binary_tree/array_representation/treemath.rs', lines 402:4-406:5 -/
+    Source: 'openmls/src/binary_tree/array_representation/treemath.rs', lines 420:4-424:5 -/
 @[rust_loop_body]
 def binary_tree.array_representation.treemath.direct_path_loop.body
   (r : Std.U32)
@@ -1128,7 +1017,7 @@ def binary_tree.array_representation.treemath.direct_path_loop.body
   else ok (done d)
 
 /-- [openmls::binary_tree::array_representation::treemath::direct_path]: loop 0:
-    Source: 'openmls/src/binary_tree/array_representation/treemath.rs', lines 402:4-406:5 -/
+    Source: 'openmls/src/binary_tree/array_representation/treemath.rs', lines 420:4-424:5 -/
 @[rust_loop]
 def binary_tree.array_representation.treemath.direct_path_loop
   (r : Std.U32)
@@ -1143,7 +1032,7 @@ def binary_tree.array_representation.treemath.direct_path_loop
     (d, x)
 
 /-- [openmls::binary_tree::array_representation::treemath::direct_path]:
-    Source: 'openmls/src/binary_tree/array_representation/treemath.rs', lines 397:0-408:1 -/
+    Source: 'openmls/src/binary_tree/array_representation/treemath.rs', lines 415:0-426:1 -/
 def binary_tree.array_representation.treemath.direct_path
   (node_index : binary_tree.array_representation.treemath.LeafNodeIndex)
   (size : binary_tree.array_representation.treemath.TreeSize) :
@@ -1160,7 +1049,7 @@ def binary_tree.array_representation.treemath.direct_path
   binary_tree.array_representation.treemath.direct_path_loop r d x
 
 /-- [openmls::binary_tree::array_representation::treemath::copath]: loop body 0:
-    Source: 'openmls/src/binary_tree/array_representation/treemath.rs', lines 425:4-427:5 -/
+    Source: 'openmls/src/binary_tree/array_representation/treemath.rs', lines 438:4-440:5 -/
 @[rust_loop_body]
 def binary_tree.array_representation.treemath.copath_loop.body
   (iter : core.slice.iter.Iter
@@ -1183,7 +1072,7 @@ def binary_tree.array_representation.treemath.copath_loop.body
     ok (cont (iter1, full_path1))
 
 /-- [openmls::binary_tree::array_representation::treemath::copath]: loop 0:
-    Source: 'openmls/src/binary_tree/array_representation/treemath.rs', lines 425:4-427:5 -/
+    Source: 'openmls/src/binary_tree/array_representation/treemath.rs', lines 438:4-440:5 -/
 @[rust_loop]
 def binary_tree.array_representation.treemath.copath_loop
   (iter : core.slice.iter.Iter
@@ -1200,7 +1089,7 @@ def binary_tree.array_representation.treemath.copath_loop
     (iter, full_path)
 
 /-- [openmls::binary_tree::array_representation::treemath::copath]:
-    Source: 'openmls/src/binary_tree/array_representation/treemath.rs', lines 417:0-429:1 -/
+    Source: 'openmls/src/binary_tree/array_representation/treemath.rs', lines 430:0-442:1 -/
 def binary_tree.array_representation.treemath.copath
   (leaf_index : binary_tree.array_representation.treemath.LeafNodeIndex)
   (size : binary_tree.array_representation.treemath.TreeSize) :
@@ -1247,7 +1136,7 @@ def binary_tree.array_representation.treemath.copath
     binary_tree.array_representation.treemath.TreeNodeIndex) m
 
 /-- [openmls::binary_tree::array_representation::treemath::lowest_common_ancestor]: loop body 0:
-    Source: 'openmls/src/binary_tree/array_representation/treemath.rs', lines 446:4-450:5 -/
+    Source: 'openmls/src/binary_tree/array_representation/treemath.rs', lines 459:4-463:5 -/
 @[rust_loop_body]
 def binary_tree.array_representation.treemath.lowest_common_ancestor_loop0.body
   (xn : Std.U32) (yn : Std.U32) (k : Std.I32) :
@@ -1262,7 +1151,7 @@ def binary_tree.array_representation.treemath.lowest_common_ancestor_loop0.body
   else ok (done (xn, k))
 
 /-- [openmls::binary_tree::array_representation::treemath::lowest_common_ancestor]: loop 0:
-    Source: 'openmls/src/binary_tree/array_representation/treemath.rs', lines 446:4-450:5 -/
+    Source: 'openmls/src/binary_tree/array_representation/treemath.rs', lines 459:4-463:5 -/
 @[rust_loop]
 def binary_tree.array_representation.treemath.lowest_common_ancestor_loop0
   (xn : Std.U32) (yn : Std.U32) (k : Std.I32) :
@@ -1275,7 +1164,7 @@ def binary_tree.array_representation.treemath.lowest_common_ancestor_loop0
     (xn, yn, k)
 
 /-- [openmls::binary_tree::array_representation::treemath::lowest_common_ancestor]: loop body 1:
-    Source: 'openmls/src/binary_tree/array_representation/treemath.rs', lines 446:4-450:5 -/
+    Source: 'openmls/src/binary_tree/array_representation/treemath.rs', lines 459:4-463:5 -/
 @[rust_loop_body]
 def binary_tree.array_representation.treemath.lowest_common_ancestor_loop1.body
   (xn : Std.U32) (yn : Std.U32) (k : Std.I32) :
@@ -1290,7 +1179,7 @@ def binary_tree.array_representation.treemath.lowest_common_ancestor_loop1.body
   else ok (done (xn, k))
 
 /-- [openmls::binary_tree::array_representation::treemath::lowest_common_ancestor]: loop 1:
-    Source: 'openmls/src/binary_tree/array_representation/treemath.rs', lines 446:4-450:5 -/
+    Source: 'openmls/src/binary_tree/array_representation/treemath.rs', lines 459:4-463:5 -/
 @[rust_loop]
 def binary_tree.array_representation.treemath.lowest_common_ancestor_loop1
   (xn : Std.U32) (yn : Std.U32) (k : Std.I32) :
@@ -1303,7 +1192,7 @@ def binary_tree.array_representation.treemath.lowest_common_ancestor_loop1
     (xn, yn, k)
 
 /-- [openmls::binary_tree::array_representation::treemath::lowest_common_ancestor]: loop body 2:
-    Source: 'openmls/src/binary_tree/array_representation/treemath.rs', lines 446:4-450:5 -/
+    Source: 'openmls/src/binary_tree/array_representation/treemath.rs', lines 459:4-463:5 -/
 @[rust_loop_body]
 def binary_tree.array_representation.treemath.lowest_common_ancestor_loop2.body
   (xn : Std.U32) (yn : Std.U32) (k : Std.I32) :
@@ -1318,7 +1207,7 @@ def binary_tree.array_representation.treemath.lowest_common_ancestor_loop2.body
   else ok (done (xn, k))
 
 /-- [openmls::binary_tree::array_representation::treemath::lowest_common_ancestor]: loop 2:
-    Source: 'openmls/src/binary_tree/array_representation/treemath.rs', lines 446:4-450:5 -/
+    Source: 'openmls/src/binary_tree/array_representation/treemath.rs', lines 459:4-463:5 -/
 @[rust_loop]
 def binary_tree.array_representation.treemath.lowest_common_ancestor_loop2
   (xn : Std.U32) (yn : Std.U32) (k : Std.I32) :
@@ -1331,7 +1220,7 @@ def binary_tree.array_representation.treemath.lowest_common_ancestor_loop2
     (xn, yn, k)
 
 /-- [openmls::binary_tree::array_representation::treemath::lowest_common_ancestor]: loop body 3:
-    Source: 'openmls/src/binary_tree/array_representation/treemath.rs', lines 446:4-450:5 -/
+    Source: 'openmls/src/binary_tree/array_representation/treemath.rs', lines 459:4-463:5 -/
 @[rust_loop_body]
 def binary_tree.array_representation.treemath.lowest_common_ancestor_loop3.body
   (xn : Std.U32) (yn : Std.U32) (k : Std.I32) :
@@ -1346,7 +1235,7 @@ def binary_tree.array_representation.treemath.lowest_common_ancestor_loop3.body
   else ok (done (xn, k))
 
 /-- [openmls::binary_tree::array_representation::treemath::lowest_common_ancestor]: loop 3:
-    Source: 'openmls/src/binary_tree/array_representation/treemath.rs', lines 446:4-450:5 -/
+    Source: 'openmls/src/binary_tree/array_representation/treemath.rs', lines 459:4-463:5 -/
 @[rust_loop]
 def binary_tree.array_representation.treemath.lowest_common_ancestor_loop3
   (xn : Std.U32) (yn : Std.U32) (k : Std.I32) :
@@ -1359,7 +1248,7 @@ def binary_tree.array_representation.treemath.lowest_common_ancestor_loop3
     (xn, yn, k)
 
 /-- [openmls::binary_tree::array_representation::treemath::lowest_common_ancestor]:
-    Source: 'openmls/src/binary_tree/array_representation/treemath.rs', lines 434:0-452:1 -/
+    Source: 'openmls/src/binary_tree/array_representation/treemath.rs', lines 447:0-465:1 -/
 def binary_tree.array_representation.treemath.lowest_common_ancestor
   (x : binary_tree.array_representation.treemath.LeafNodeIndex)
   (y : binary_tree.array_representation.treemath.LeafNodeIndex) :
@@ -1445,7 +1334,7 @@ def binary_tree.array_representation.treemath.lowest_common_ancestor
         i6
 
 /-- [openmls::binary_tree::array_representation::treemath::common_direct_path]: loop body 0:
-    Source: 'openmls/src/binary_tree/array_representation/treemath.rs', lines 475:4-484:5 -/
+    Source: 'openmls/src/binary_tree/array_representation/treemath.rs', lines 483:4-492:5 -/
 @[rust_loop_body]
 def binary_tree.array_representation.treemath.common_direct_path_loop.body
   (x_path : alloc.vec.Vec
@@ -1480,7 +1369,7 @@ def binary_tree.array_representation.treemath.common_direct_path_loop.body
   else ok (done common_path)
 
 /-- [openmls::binary_tree::array_representation::treemath::common_direct_path]: loop 0:
-    Source: 'openmls/src/binary_tree/array_representation/treemath.rs', lines 475:4-484:5 -/
+    Source: 'openmls/src/binary_tree/array_representation/treemath.rs', lines 483:4-492:5 -/
 @[rust_loop]
 def binary_tree.array_representation.treemath.common_direct_path_loop
   (x_path : alloc.vec.Vec
@@ -1499,7 +1388,7 @@ def binary_tree.array_representation.treemath.common_direct_path_loop
     (common_path, i)
 
 /-- [openmls::binary_tree::array_representation::treemath::common_direct_path]:
-    Source: 'openmls/src/binary_tree/array_representation/treemath.rs', lines 462:0-488:1 -/
+    Source: 'openmls/src/binary_tree/array_representation/treemath.rs', lines 470:0-496:1 -/
 def binary_tree.array_representation.treemath.common_direct_path
   (x : binary_tree.array_representation.treemath.LeafNodeIndex)
   (y : binary_tree.array_representation.treemath.LeafNodeIndex)
@@ -1532,7 +1421,7 @@ def binary_tree.array_representation.treemath.common_direct_path
   ok (deref_mut_back2 s5)
 
 /-- [openmls::binary_tree::array_representation::treemath::is_node_in_tree]:
-    Source: 'openmls/src/binary_tree/array_representation/treemath.rs', lines 503:0-505:1 -/
+    Source: 'openmls/src/binary_tree/array_representation/treemath.rs', lines 508:0-510:1 -/
 def binary_tree.array_representation.treemath.is_node_in_tree
   (node_index : binary_tree.array_representation.treemath.TreeNodeIndex)
   (size : binary_tree.array_representation.treemath.TreeSize) :
